
%Let $\vq^*(t)=\vq(t)+\delta\vq(t)$, where $\delta\vq(t)$ is a small variation. It must satisfy
%\begin{gather}
%	\suman a^*_{k\alpha}\md q^*_\alpha+a^*_{kt}\md t=0
%	\label{eq:lag-multiplier2}
%\end{gather}
%where
%\begin{align*}
%	a^*_{k\alpha}&=\p{\sigma_k}{q^*_\alpha}=\p{\sigma_k}{q_\alpha}\der{q_\alpha}{q^*_\alpha}\\
%	a^*_{kt}&=\p{\sigma_k}{t}=a_{kt}
%\end{align*}
%since $\delta\vq$ is independent of $\vq$, $\der{q^*_\alpha}{q_\alpha}=1+\der{\delta q_\alpha}{q_\alpha}=1$, thus
%\begin{equation*}
%	a^*_{k\alpha}=a_{k\alpha}
%\end{equation*}
%Substract eqn. \ref{eq:lag-multiplier} from \ref{eq:lag-multiplier2}, we get
%which leads to
%\begin{equation}
%	\suman a_{k\alpha}\md(q^*_\alpha-q_\alpha)=\suman a_{k\alpha}\delta\vq_\alpha=0 \label{eq:lag-multiplier}
%\end{equation}